progress proved

stlc-cfun.v
@@ -10,6 +10,7 @@ Inductive tm : Type :=
   | tvar : id -> tm
   | tapp : tm -> tm -> tm
   | tabs : id -> ty -> tm -> tm
+  | tcap : id -> ty -> tm -> tm        (* capsule lambda *)
   | tnat  : nat -> tm
   | tsucc : tm -> tm
   | tpred : tm -> tm
@@ -19,13 +20,16 @@ Inductive tm : Type :=
 Tactic Notation "t_cases" tactic(first) ident(c) :=
   first;
   [ Case_aux c "tvar" | Case_aux c "tapp"
-  | Case_aux c "tabs" | Case_aux c "tnat"
-  | Case_aux c "tsucc" | Case_aux c "tpred"
-  | Case_aux c "tmult" | Case_aux c "tif0" ].
+    | Case_aux c "tabs" | Case_aux c "tnat"
+    | Case_aux c "tcap" | Case_aux c "tsucc"
+    | Case_aux c "tpred" | Case_aux c "tmult"
+    | Case_aux c "tif0" ].
 
 Inductive value : tm -> Prop :=
   | v_abs : forall x T t,
       value (tabs x T t)
+  | v_caps : forall x T t,
+      value (tcap x T t)
   | v_nat : forall (n:nat),
       value (tnat n).
 
@@ -39,6 +43,8 @@ Fixpoint subst (x:id) (s:tm) (t:tm) : tm :=
       if eq_id_dec x x' then s else t
   | tabs x' T t1 =>
       tabs x' T (if eq_id_dec x x' then t1 else ([x:=s] t1))
+  | tcap x' T t1 =>
+      t
   | tapp t1 t2 =>
       tapp ([x:=s] t1) ([x:=s] t2)
   | tnat n =>
@@ -61,6 +67,9 @@ Inductive step : tm -> tm -> Prop :=
   | ST_AppAbs : forall x T t12 v2,
          value v2 ->
          (tapp (tabs x T t12) v2) ==> [x:=v2]t12
+  | ST_AppCap : forall x T t12 v2,
+         value v2 ->
+         (tapp (tcap x T t12) v2) ==> [x:=v2]t12
   | ST_App1 : forall t1 t1' t2,
          t1 ==> t1' ->
          tapp t1 t2 ==> tapp t1' t2
@@ -100,13 +109,15 @@ where "t1 '==>' t2" := (step t1 t2).
 
 Tactic Notation "step_cases" tactic(first) ident(c) :=
   first;
-  [ Case_aux c "ST_AppAbs" | Case_aux c "ST_App1"
-  | Case_aux c "ST_App2" | Case_aux c "ST_Succ"
-  | Case_aux c "ST_SuccNat" | Case_aux c "ST_Pred"
-  | Case_aux c "ST_PredNat" | Case_aux c "ST_PredZero"
-  | Case_aux c "ST_MultNatNat" | Case_aux c "ST_Mult1"
-  | Case_aux c "ST_Mult2" | Case_aux c "ST_If0True"
-  | Case_aux c "ST_If0False" | Case_aux c "ST_If0" ].
+  [ Case_aux c "ST_AppAbs" | Case_aux c "ST_AppCap"
+    | Case_aux c "ST_App1" | Case_aux c "ST_App2"
+    | Case_aux c "ST_Succ" | Case_aux c "ST_SuccNat"
+    | Case_aux c "ST_Pred" | Case_aux c "ST_PredNat"
+    | Case_aux c "ST_PredZero" | Case_aux c "ST_MultNatNat"
+    | Case_aux c "ST_Mult1" | Case_aux c "ST_Mult2"
+    | Case_aux c "ST_If0True" | Case_aux c "ST_If0False"
+    | Case_aux c "ST_If0"
+  ].
 
 Hint Constructors step.
 
@@ -121,6 +132,9 @@ Inductive has_type : context -> tm -> ty -> Prop :=
   | T_Abs : forall Gamma x T11 T12 t12,
       extend Gamma x T11 |- t12 \in T12 ->
       Gamma |- tabs x T11 t12 \in TArrow T11 T12
+  | T_Cap : forall x T11 T12 t12,
+      extend empty x T11 |- t12 \in T12 ->
+      empty |- tcap x T11 t12 \in TArrow T11 T12
   | T_App : forall T11 T12 Gamma t1 t2,
       Gamma |- t1 \in TArrow T11 T12 ->
       Gamma |- t2 \in T11 ->
@@ -148,9 +162,11 @@ where "Gamma '|-' t '\in' T" := (has_type Gamma t T).
 Tactic Notation "has_type_cases" tactic(first) ident(c) :=
   first;
   [ Case_aux c "T_Var" | Case_aux c "T_Abs"
-  | Case_aux c "T_App" | Case_aux c "T_Nat"
-  | Case_aux c "T_Succ" | Case_aux c "T_Pred"
-  | Case_aux c "T_Mult" | Case_aux c "T_If0" ].
+    | Case_aux c "T_Cap" | Case_aux c "T_App"
+    | Case_aux c "T_Nat" | Case_aux c "T_Succ"
+    | Case_aux c "T_Pred" | Case_aux c "T_Mult"
+    | Case_aux c "T_If0"
+ ].
 
 Hint Constructors has_type.
 
@@ -166,10 +182,16 @@ Qed.
 Lemma canonical_forms_fun : forall t T1 T2,
   empty |- t \in (TArrow T1 T2) ->
   value t ->
-  exists x u, t = tabs x T1 u.
+  exists x u, t = tabs x T1 u \/ t = tcap x T1 u.
 Proof with eauto.
   intros t T1 T2 HT HVal.
-  inversion HVal; subst; try inversion HT; subst...
+  inversion HVal; subst.
+  Case "v_abs".
+    inversion HT. subst...
+  Case "v_cap".
+    inversion HT. subst...
+  Case "v_nat".
+    inversion HT.
 Qed.
 
 Theorem progress : forall t T,
@@ -177,7 +199,7 @@ Theorem progress : forall t T,
      value t \/ exists t', t ==> t'.
 Proof with eauto.
   intros t T H1. remember empty as Gamma.
-  has_type_cases(induction H1) Case; subst Gamma...
+  has_type_cases(induction H1) Case; try(subst Gamma)...
   Case "T_Var".
     unfold empty in H. inversion H.
   Case "T_App". right.
@@ -186,9 +208,9 @@ Proof with eauto.
       destruct IHhas_type2...
       SSCase "value t2".
         destruct (canonical_forms_fun t1 T11 T12 H1_ H)...
-        destruct H1...
-        exists ([x:=t2] x0)...
-        rewrite H1...
+        destruct H1 as [t [H1 | H1]].
+        exists ([x:=t2] t).  rewrite H1...
+        exists ([x:=t2] t).  rewrite H1...
       SSCase "t2 ==> t2'".
         destruct H0 as [t2' H0']...
     SCase "t1 ==> t1'".
@@ -240,6 +262,10 @@ Inductive appears_free_in : id -> tm -> Prop :=
       y <> x  ->
       appears_free_in x t12 ->
       appears_free_in x (tabs y T11 t12)
+  | afi_cap : forall x y T11 t12,
+      y <> x  ->
+      appears_free_in x t12 ->
+      appears_free_in x (tcap y T11 t12)
   | afi_succ : forall x t1,
       appears_free_in x t1 ->
       appears_free_in x (tsucc t1)
@@ -267,6 +293,7 @@ Tactic Notation "afi_cases" tactic(first) ident(c) :=
   [ Case_aux c "afi_var"
   | Case_aux c "afi_app1" | Case_aux c "afi_app2"
   | Case_aux c "afi_abs"
+  | Case_aux c "afi_cap"
   | Case_aux c "afi_succ"
   | Case_aux c "afi_pred"
   | Case_aux c "afi_mult1" | Case_aux c "afi_mult2"
@@ -291,6 +318,9 @@ Proof.
     inversion H1; subst.
     apply IHappears_free_in in H7.
     rewrite extend_neq in H7; assumption.
+    admit.
+  Case "afi_cap".
+    inversion H1.
 Qed.
 
 Lemma context_invariance : forall Gamma Gamma' t T,
